correctness of compile_labels

compiler/correctness/compileCorrectnessScript.sml
@@ -1,6 +1,5 @@
-open HolKernel bossLib boolLib boolSimps SatisfySimps listTheory pairTheory pred_setTheory finite_mapTheory alistTheory relationTheory lcsymtacs
-open MiniMLTerminationTheory miniMLExtraTheory miscTheory compileTerminationTheory intLangTheory bytecodeTerminationTheory evaluateEquationsTheory expToCexpTheory quantHeuristicsLib
-open pmatchTheory labelClosuresTheory
+open HolKernel bossLib boolLib boolSimps SatisfySimps listTheory rich_listTheory pairTheory pred_setTheory finite_mapTheory alistTheory relationTheory lcsymtacs quantHeuristicsLib
+open MiniMLTerminationTheory miniMLExtraTheory miscTheory compileTerminationTheory intLangTheory bytecodeTerminationTheory evaluateEquationsTheory expToCexpTheory pmatchTheory labelClosuresTheory bytecodeEvalTheory
 val _ = intLib.deprecate_int()
 val _ = new_theory "compileCorrectness"
 
@@ -312,7 +311,7 @@ val INJ_has_fmap_linv = store_thm("INJ_has_fmap_linv",
 
 val has_fmap_linv_inj = store_thm("has_fmap_linv_inj",
   ``(?g. fmap_linv f g) = (INJ (FAPPLY f) (FDOM f) (FRANGE f))``,
-  REVERSE EQ_TAC THEN1 PROVE_TAC[INJ_has_fmap_linv] THEN
+  Tactical.REVERSE EQ_TAC THEN1 PROVE_TAC[INJ_has_fmap_linv] THEN
   SRW_TAC[][fmap_linv_def,INJ_DEF,EQ_IMP_THM]
   THEN1 ( SRW_TAC[][FRANGE_DEF] THEN PROVE_TAC[] )
   THEN1 ( FULL_SIMP_TAC(srw_ss())[FLOOKUP_DEF] THEN PROVE_TAC[] ))
@@ -386,6 +385,11 @@ val el_of_addr_def = Define`
        if n < il x + 1 then NONE else
          OPTION_BIND (el_of_addr il (n - (il x + 1)) xs) (λm. SOME (m + 1)))`
 val _ = export_rewrites["el_of_addr_def"]
+
+val el_of_addr_LESS_LENGTH = store_thm("el_of_addr_LESS_LENGTH",
+  ``∀il ls n m. (el_of_addr il n ls = SOME m) ⇒ m < LENGTH ls``,
+  gen_tac >> Induct >> srw_tac[ARITH_ss][] >>
+  res_tac >> fsrw_tac[ARITH_ss][])
 
 val bc_fetch_aux_el_of_addr = store_thm("bc_fetch_aux_el_of_addr",
   ``∀c il pc. bc_fetch_aux c il pc = OPTION_BIND (el_of_addr il pc c) (λn. SOME (EL n c))``,
@@ -464,17 +468,239 @@ val calculate_labels_thm = store_thm("calculate_labels_thm",
       AP_TERM_TAC >>
       rw[bc_find_loc_aux_def] )))
 
-val compile_labels_bc_next = store_thm("compile_labels_bc_next",
-  ``∀s1 s2. bc_next s1 s2 ⇒ bc_next
-      (s1 with <| code := compile_labels s1.inst_length 0 s1.code |>)
-      (s2 with <| code := compile_labels s2.inst_length 0 s2.code |>)``,
-  compile_labels_def
-  TypeBase.fields_of``:bc_state``
-  compile
+val replace_lab_def = Define`
+  (replace_lab m (Jump (Lab l)) = Jump (Addr (FAPPLY m l))) ∧
+  (replace_lab m (JumpIf (Lab l)) = JumpIf (Addr (m ' l))) ∧
+  (replace_lab m (Call (Lab l)) = Call (Addr (m ' l))) ∧
+  (replace_lab m (PushPtr (Lab l)) = PushPtr (Addr (m ' l))) ∧
+  (replace_lab m i = i)`
+val _ = export_rewrites["replace_lab_def"]
+
+val replace_labels_thm = store_thm("replace_labels_thm",
+  ``∀m a ls. (replace_labels m a ls = (REVERSE (MAP (replace_lab m) ls)) ++ a)``,
+  ho_match_mp_tac replace_labels_ind >> rw[replace_labels_def])
+
+val bc_fetch_aux_MAP = store_thm("bc_fetch_aux_MAP",
+  ``!il f. (∀x. il (f x) = il x) ∧ (∀x. is_Label (f x) = is_Label x) ⇒
+      ∀ls n. (bc_fetch_aux (MAP f ls) il n = OPTION_MAP f (bc_fetch_aux ls il n))``,
+  ntac 2 gen_tac >> strip_tac >>
+  Induct >> rw[bc_fetch_aux_def])
+
+val bc_fetch_MAP = store_thm("bc_fetch_MAP",
+  ``∀f s. (∀x. s.inst_length (f x) = s.inst_length x) ∧ (∀x. is_Label (f x) = is_Label x) ⇒
+    (bc_fetch (s with <| code := MAP f s.code |>) = OPTION_MAP f (bc_fetch s))``,
+  rw[bc_fetch_def,bc_fetch_aux_MAP])
+
+val is_Label_replace_lab = store_thm("is_Label_replace_lab",
+  ``∀x. is_Label (replace_lab m x) = is_Label x``,
+  Cases >> rw[] >> Cases_on `l` >> rw[])
+val _ = export_rewrites["is_Label_replace_lab"]
+
+val good_il_def = Define`
+  good_il il =
+  (∀x. il (Jump x) = il (Jump ARB)) ∧
+  (∀x. il (JumpIf x) = il (JumpIf ARB)) ∧
+  (∀x. il (Call x) = il (Call ARB)) ∧
+  (∀x. il (PushPtr x) = il (PushPtr ARB))`
+
+val il_replace_lab = store_thm("il_replace_lab",
+  ``good_il il ⇒ ∀m x. (il (replace_lab m x) = il x)``,
+  rw[good_il_def] >>
+  Cases_on `x` >> rw[] >>
+  Cases_on `l` >> rw[])
+
+val bc_fetch_with_stack = store_thm("bc_fetch_with_stack",
+  ``bc_fetch (s with stack := st) = bc_fetch s``,
+  rw[bc_fetch_def])
+
+val bump_pc_with_stack = store_thm("bump_pc_with_stack",
+  ``bump_pc (s with stack := st) = (bump_pc s) with stack := st``,
+  rw[bump_pc_def,bc_fetch_with_stack] >>
+  BasicProvers.EVERY_CASE_TAC)
+
+val tac = (
+    rw[LET_THM] >>
+    match_mp_tac bc_eval1_SOME >>
+    Q.PAT_ABBREV_TAC`f = replace_lab X` >>
+    qspecl_then[`f`,`s1`] mp_tac bc_fetch_MAP >>
+    qunabbrev_tac`f` >> rw[il_replace_lab] >>
+    rw[bc_eval1_def] >>
+    fs[bc_eval_stack_thm] >>
+    fs[bump_pc_def] )
+
+val tac2 = (
+    rw[LET_THM] >>
+    match_mp_tac bc_eval1_SOME >>
+    Q.PAT_ABBREV_TAC`f = replace_lab X` >>
+    qspecl_then[`f`,`s1`] mp_tac bc_fetch_MAP >>
+    qunabbrev_tac`f` >>
+    Cases_on `l` >> rw[il_replace_lab] >>
+    srw_tac[DNF_ss][bc_eval1_def,LET_THM] >>
+    fs[bc_eval_stack_thm,bc_find_loc_def] >>
+    fs[FLOOKUP_DEF] >>
+    rw[bump_pc_with_stack] >>
+    rw[bump_pc_def] >>
+    fs[good_il_def] >>
+    metis_tac[optionTheory.SOME_11,optionTheory.NOT_SOME_NONE])
+
+val bc_next_MAP_replace_lab = store_thm("bc_next_MAP_replace_lab",
+  ``∀s1 s2. bc_next s1 s2 ⇒
+      ∀m. good_il s1.inst_length ∧
+      (∀l. FLOOKUP m l = bc_find_loc s1 (Lab l)) ⇒
+    let c = MAP (replace_lab m) s1.code in
+    bc_next (s1 with <| code := c |>) (s2 with <| code := c |>)``,
+  ho_match_mp_tac bc_next_ind >>
+  strip_tac >- tac >>
+  strip_tac >- tac2 >>
+  strip_tac >- tac2 >>
+  strip_tac >- tac2 >>
+  strip_tac >- tac >>
+  strip_tac >- tac >>
+  strip_tac >- tac2 >>
+  strip_tac >- tac >>
+  strip_tac >- tac >>
+  strip_tac >- tac >>
+  strip_tac >- tac >>
+  strip_tac >- tac )
+
+val labels_only_def = Define`
+  (labels_only (Jump (Addr _)) = F) ∧
+  (labels_only (JumpIf (Addr _)) = F) ∧
+  (labels_only (Call (Addr _)) = F) ∧
+  (labels_only (PushPtr (Addr _)) = F) ∧
+  (labels_only _ = T)`
+val _ = export_rewrites["labels_only_def"]
+
+val addrs_only_def = Define`
+  (addrs_only (Jump (Lab _)) = F) ∧
+  (addrs_only (JumpIf (Lab _)) = F) ∧
+  (addrs_only (Call (Lab _)) = F) ∧
+  (addrs_only (PushPtr (Lab _)) = F) ∧
+  (addrs_only _ = T)`
+val _ = export_rewrites["addrs_only_def"]
+
+val bc_fetch_aux_FILTER_labels = store_thm("bc_fetch_aux_FILTER_labels",
+  ``∀il ls n. bc_fetch_aux (FILTER ($~ o is_Label) ls) il n = bc_fetch_aux ls il n``,
+  gen_tac >> Induct >> rw[])
+val _ = export_rewrites["bc_fetch_aux_FILTER_labels"]
+
+val bc_fetch_FILTER_labels = store_thm("bc_fetch_FILTER_labels",
+  ``bc_fetch (s with code := FILTER ($~ o is_Label) s.code) = bc_fetch s``,
+  rw[bc_fetch_def])
+val _ = export_rewrites["bc_fetch_FILTER_labels"]
+
+val bc_fetch_MEM = store_thm("bc_fetch_MEM",
+  ``(bc_fetch s1 = SOME i) ⇒ (MEM i s1.code)``,
+  rw[bc_fetch_def] >>
+  fs[bc_fetch_aux_el_of_addr] >>
+  rw[MEM_EL] >>
+  imp_res_tac el_of_addr_LESS_LENGTH >>
+  metis_tac[])
+
+val bc_next_FILTER_labels = store_thm("bc_next_FILTER",
+  ``∀s1 s2. bc_next s1 s2 ⇒ EVERY addrs_only s1.code ⇒
+      let c = FILTER ($~ o is_Label) s1.code in
+      bc_next (s1 with <| code := c |>) (s2 with <| code := c |>)``,
+  ho_match_mp_tac bc_next_ind >>
+  rw[LET_THM] >>
+  rw[bc_eval1_thm] >>
+  srw_tac[DNF_ss][bc_eval1_def,LET_THM] >>
+  fs[bc_eval_stack_thm] >>
+  rw[bump_pc_def] >>
+  imp_res_tac bc_fetch_MEM >>
+  fs[EVERY_MEM] >>
+  res_tac >>
+  Cases_on `l` >> fs[bc_find_loc_def] >>
+  rw[bc_fetch_with_stack])
+
+val addrs_only_replace_lab = store_thm("addrs_only_replace_lab",
+  ``addrs_only (replace_lab m x)``,
+  Cases_on `x` >> rw[] >> Cases_on `l` >> rw[])
+val _ = export_rewrites["addrs_only_replace_lab"]
+
+val bc_find_loc_aux_NONE = store_thm("bc_find_loc_aux_NONE",
+  ``∀il l ls n. (bc_find_loc_aux ls il l n = NONE) ⇒ ¬MEM (Label l) ls``,
+  ntac 2 gen_tac >>
+  Induct >> rw[bc_find_loc_aux_def] >>
+  res_tac >> fs[])
+
+val bc_find_loc_aux_MEM = store_thm("bc_find_loc_aux_MEM",
+  ``∀il l ls n. (bc_find_loc_aux ls il l n ≠ NONE) ⇒ MEM (Label l) ls``,
+  ntac 2 gen_tac >>
+  Induct >> rw[bc_find_loc_aux_def] >>
+  res_tac)
+
+(* TODO: move *)
+val ALL_DISTINCT_MAP_INJ = store_thm("ALL_DISTINCT_MAP_INJ",
+  ``!ls f. (!x y. MEM x ls /\ MEM y ls /\ (f x = f y) ==> (x = y)) /\ ALL_DISTINCT ls  ==> ALL_DISTINCT (MAP f ls)``,
+  Induct THEN SRW_TAC[][MEM_MAP] THEN PROVE_TAC[])
+
+val bc_next_compile_labels = store_thm("bc_next_compile_labels",
+  ``∀s1 s2. bc_next s1 s2 ⇒
+      (good_il s1.inst_length ∧
+       ALL_DISTINCT (FILTER is_Label s1.code)) ⇒
+      let c = compile_labels s1.inst_length 0 s1.code in
+      bc_next (s1 with <| code := c |>) (s2 with <| code := c |>)``,
+  rw[compile_labels_def,replace_labels_thm] >>
+  imp_res_tac calculate_labels_thm >>
+  rpt BasicProvers.VAR_EQ_TAC >>
+  qunabbrev_tac`c` >>
+  rw[MAP_REVERSE] >>
+  `∀x. ($~ o is_Label) (replace_lab m x) = ($~ o is_Label) x` by rw[] >>
+  rw[MAP_FILTER] >>
+  qmatch_abbrev_tac `bc_next (s1 with code := FILTER P ls) (s2 with code := FILTER P ls)` >>
+  `EVERY addrs_only ls` by (
+    qunabbrev_tac`ls` >>
+    rw[EVERY_MAP] ) >>
+  `bc_next (s1 with code := ls) (s2 with code := ls)` by (
+    qunabbrev_tac`ls` >>
+    match_mp_tac (MP_CANON(SIMP_RULE(srw_ss())[LET_THM]bc_next_MAP_replace_lab)) >>
+    rw[bc_find_loc_def] >>
+    fs[LET_THM] >>
+    qmatch_abbrev_tac `FLOOKUP (fm |++ ls) l = X` >>
+    Cases_on `X` >- (
+      `ALOOKUP (REVERSE ls) l = NONE` by (
+        qunabbrev_tac`ls` >>
+        rw[ALOOKUP_FAILS,ZIP_MAP] >>
+        rw[MAP_MAP_o,combinTheory.o_DEF] >>
+        `¬MEM (Label l) s1.code` by metis_tac[bc_find_loc_aux_NONE] >>
+        `¬MEM (Label l) (FILTER is_Label s1.code)` by rw[MEM_FILTER] >>
+        rw[MEM_MAP] >>
+        Cases_on `x` >> rw[MEM_FILTER] >>
+        PROVE_TAC[] ) >>
+      imp_res_tac FLOOKUP_FUPDATE_LIST_ALOOKUP_NONE >>
+      fs[Abbr`fm`] ) >>
+    `ALOOKUP (REVERSE ls) l = SOME x` by (
+      match_mp_tac ALOOKUP_ALL_DISTINCT_MEM >>
+      qunabbrev_tac`ls` >>
+      rw[REVERSE_ZIP,MAP_ZIP,ALL_DISTINCT_REVERSE] >- (
+        match_mp_tac ALL_DISTINCT_MAP_INJ >> fs[] >>
+        qx_gen_tac `a` >> qx_gen_tac `b` >>
+        Cases_on `a` >> Cases_on `b` >> rw[MEM_FILTER] ) >>
+      `MEM (Label l) s1.code` by
+        metis_tac[bc_find_loc_aux_MEM,optionTheory.NOT_SOME_NONE] >>
+      `MEM (Label l) (FILTER is_Label s1.code)` by rw[MEM_FILTER] >>
+      pop_assum (strip_assume_tac o SIMP_RULE (srw_ss()) [MEM_EL]) >>
+      rw[MEM_ZIP] >>
+      qexists_tac `n` >>
+      pop_assum (assume_tac o SYM) >>
+      rw[EL_MAP] ) >>
+    imp_res_tac FLOOKUP_FUPDATE_LIST_ALOOKUP_SOME >>
+    fs[] ) >>
+  qunabbrev_tac`P` >>
+  `ls = (s1 with code := ls).code` by rw[] >>
+  pop_assum SUBST1_TAC >>
+  (bc_next_FILTER_labels
+   |> SIMP_RULE std_ss [LET_THM]
+   |> Q.SPECL[`s1 with code := ls`,`s2 with code := ls`]
+   |> SIMP_RULE (srw_ss()) []
+   |> MP_CANON |> match_mp_tac ) >>
+  fs[])
 
 val next_addr_def = Define`
   next_addr bs = FST(SND(calculate_labels bs.inst_length FEMPTY 0 [] bs.code))`
 
+(*
 val repl_exp_val = store_thm("repl_exp_val",
   ``∀cenv env exp v rs rs' bc bs bs'.
       exp_pred exp ∧
@@ -511,14 +737,7 @@ val repl_exp_val = store_thm("repl_exp_val",
   fs[] >>
   fs[calculate_ecs_def] >>
   fs[compile_code_env_def,LET_THM] >>
-
-val labels_only_def = Define`
-  labels_only ls = ∀x. MEM x ls ⇒ case x of
-    | Jump (Addr _) => F
-    | JumpIf (Addr _) => F
-    | Call (Addr _) => F
-    | PushPtr (Addr _) => F
-    | _ => T`;
+*)
 
 val with_same_pc = store_thm("with_same_pc",
   ``x with pc := x.pc = x``,
